# Relativity

## General Relativity

### Equations

\[

\begin{align*}

v^\alpha &= \frac{d}{d\tau} x^\alpha\\

\vec{v} &= v^\alpha \vec{e}_\alpha \\

||\vec{v}|| &= c \\

\frac{d}{d\tau} \vec{v} &= \vec{0} \\

\frac{d}{dx^\beta} \vec{e}_\alpha &= \Gamma^\gamma{}_{\alpha\beta} \vec{e}_\gamma \\

\frac{d}{d\tau} v^\alpha &= -\Gamma^\alpha{}_{\mu\nu} v^\mu v^\nu \\

g^{\mu\nu} &= \left(g^{-1}\right)_{\mu\nu} \\

(ds)^2 &= g_{\mu\nu} dx^\mu dx^\nu \\

||\vec{v}||^2 = c^2 &= g_{\mu\nu} v^\mu v^\nu \\

\Gamma^\gamma{}_{\alpha\beta} &= \begin{cases}
        \frac{1}{2 g_{\gamma\gamma}} \left(  \frac{dg_{\gamma\alpha}}{dx^\beta} + \frac{dg_{\gamma\beta}}{dx^\alpha}
                                            - \frac{dg_{\alpha\beta}}{dx^\gamma} \right) & \text{orthogonal basis} \\
        \frac{g^{\gamma\sigma}}{2} \left( \frac{dg_{\sigma\alpha}}{dx^\beta} + \frac{dg_{\sigma\beta}}{dx^\alpha} 
                                          - \frac{dg_{\alpha\beta}}{dx^\sigma} \right) & \text{else}\\
    \end{cases}


\end{align*}
\]
